Code beautify

AML_definition.v
@@ -12,14 +12,14 @@ Inductive SVar : Set := svar_c (id : string).
 Inductive Sigma : Set := sigma_c (id : string).
 
 Inductive Sigma_pattern : Set :=
-  | sp_var (x : EVar)
-  | sp_set (X : SVar)
-  | sp_const (sigma : Sigma)
-  | sp_app (phi1 phi2 : Sigma_pattern)
-  | sp_bottom
-  | sp_impl (phi1 phi2 : Sigma_pattern)
-  | sp_exists (x : EVar) (phi : Sigma_pattern)
-  | sp_mu (X : SVar) (phi : Sigma_pattern)
+| sp_var (x : EVar)
+| sp_set (X : SVar)
+| sp_const (sigma : Sigma)
+| sp_app (phi1 phi2 : Sigma_pattern)
+| sp_bottom
+| sp_impl (phi1 phi2 : Sigma_pattern)
+| sp_exists (x : EVar) (phi : Sigma_pattern)
+| sp_mu (X : SVar) (phi : Sigma_pattern)
 .
 
 Notation "a _._ b" := (sp_app a b) (at level 50, left associativity).
@@ -45,20 +45,27 @@ Defined.
 Fixpoint spos_accumulated (phi : Sigma_pattern) (X : SVar) (nc : nat) : bool :=
   match phi with
   | sp_var x => true
-  | sp_set Y => if (svar_eq_dec Y X)
-                then (Nat.even nc)
-                else true
+  | sp_set Y =>
+      if (svar_eq_dec Y X) then
+        (Nat.even nc)
+      else
+        true
   | sp_const sigma => true
-  | sp_app phi1 phi2 => andb (spos_accumulated phi1 X nc) (spos_accumulated phi2 X nc)
+  | sp_app phi1 phi2 =>
+      andb (spos_accumulated phi1 X nc) (spos_accumulated phi2 X nc)
   | sp_bottom => true
-  | sp_impl phi1 phi2 => andb (spos_accumulated phi1 X (S nc)) (spos_accumulated phi2 X nc)
+  | sp_impl phi1 phi2 => 
+      andb (spos_accumulated phi1 X (S nc)) (spos_accumulated phi2 X nc)
   | sp_exists x phi => spos_accumulated phi X nc
-  | sp_mu Y phi => if (svar_eq_dec Y X)
-                      then true
-                      else (spos_accumulated phi X nc)
+  | sp_mu Y phi =>
+      if (svar_eq_dec Y X) then
+        true
+      else
+        (spos_accumulated phi X nc)
 end.
 
-Fixpoint strictly_positive (phi : Sigma_pattern) (X : SVar) : bool :=  spos_accumulated phi X 0.
+Fixpoint strictly_positive (phi : Sigma_pattern) (X : SVar) : bool :=
+  spos_accumulated phi X 0.
 
 Definition sp_eq_dec : forall (x y : Sigma_pattern), { x = y } + { x <> y }.
 Proof.
@@ -72,11 +79,11 @@ Defined.
 
 Definition sp_not (phi : Sigma_pattern) := sp_impl phi sp_bottom.
 Definition sp_or  (l r : Sigma_pattern) := sp_impl (sp_not l) r.
-Definition sp_and (l r : Sigma_pattern) :=
-  sp_not (sp_or (sp_not l) (sp_not r)).
-Notation "a _&_ b" := (sp_and a b) (right associativity, at level 70). (* TODO: Check associativity level *)
+Definition sp_and (l r : Sigma_pattern) := sp_not (sp_or (sp_not l) (sp_not r)).
+Notation "a _&_ b" := (sp_and a b) (right associativity, at level 70).
 Definition sp_tatu := sp_not sp_bottom.
-Definition sp_equiv (l r : Sigma_pattern) := (sp_and (sp_impl (l) (r)) (sp_impl (l) (r))).
+Definition sp_equiv (l r : Sigma_pattern) := 
+  (sp_and (sp_impl (l) (r)) (sp_impl (l) (r))).
 Definition sp_forall (x : EVar) (phi : Sigma_pattern) :=
   sp_not (sp_exists x (sp_not phi)).
 (*nuX.phi*)
@@ -84,226 +91,202 @@ Definition sp_forall (x : EVar) (phi : Sigma_pattern) :=
 Notation "phi1 <--> phi2" := (sp_equiv phi1 phi2) (at level 100).
 
 Fixpoint e_subst_var (phi : Sigma_pattern) (psi : Sigma_pattern) (x : EVar) :=
-  match phi with
-  | sp_var x' =>
-      if evar_eq_dec x x'
-      then psi
-      else sp_var x'
-  | sp_set X => sp_set X
-  | sp_const sigma => sp_const sigma
-  | sp_app phi1 phi2 => sp_app (e_subst_var phi1 psi x)
-                                (e_subst_var phi2 psi x)
-  | sp_bottom => sp_bottom
-  | sp_impl phi1 phi2 => sp_impl (e_subst_var phi1 psi x)
-                                  (e_subst_var phi2 psi x)
-  | sp_exists x' phi' =>
-      if (evar_eq_dec x' x)
-      then sp_exists x' phi'
-      else sp_exists x' (e_subst_var phi' psi x)
-  | sp_mu X phi' => sp_mu X (e_subst_var phi' psi x)
+match phi with
+| sp_var x' =>
+    if evar_eq_dec x x'
+    then psi
+    else sp_var x'
+| sp_set X => sp_set X
+| sp_const sigma => sp_const sigma
+| sp_app phi1 phi2 => sp_app (e_subst_var phi1 psi x)
+                              (e_subst_var phi2 psi x)
+| sp_bottom => sp_bottom
+| sp_impl phi1 phi2 => sp_impl (e_subst_var phi1 psi x) (e_subst_var phi2 psi x)
+| sp_exists x' phi' =>
+    if (evar_eq_dec x' x) then
+      sp_exists x' phi'
+    else
+      sp_exists x' (e_subst_var phi' psi x)
+| sp_mu X phi' => sp_mu X (e_subst_var phi' psi x)
 end.
 
 Fixpoint e_subst_set (phi : Sigma_pattern) (psi : Sigma_pattern) (X : SVar) :=
-  match phi with
-  | sp_var x => sp_var x
-  | sp_set X' =>
-      if svar_eq_dec X X'
-      then psi
-      else sp_set X'
-  | sp_const sigma => sp_const sigma
-  | sp_app phi1 phi2 => sp_app (e_subst_set phi1 psi X)
-                                (e_subst_set phi2 psi X)
-  | sp_bottom => sp_bottom
-  | sp_impl phi1 phi2 => sp_impl (e_subst_set phi1 psi X)
-                                  (e_subst_set phi2 psi X)
-  | sp_exists x' phi' => sp_exists x' (e_subst_set phi' psi X)
-  | sp_mu X' phi' =>
-      if (svar_eq_dec X' X)
-      then sp_mu X' phi'
-      else sp_mu X' (e_subst_set phi' psi X)
+match phi with
+| sp_var x => sp_var x
+| sp_set X' =>
+    if svar_eq_dec X X' then
+      psi
+    else
+      sp_set X'
+| sp_const sigma => sp_const sigma
+| sp_app phi1 phi2 => sp_app (e_subst_set phi1 psi X) (e_subst_set phi2 psi X)
+| sp_bottom => sp_bottom
+| sp_impl phi1 phi2 => sp_impl (e_subst_set phi1 psi X) (e_subst_set phi2 psi X)
+| sp_exists x' phi' => sp_exists x' (e_subst_set phi' psi X)
+| sp_mu X' phi' => 
+    if (svar_eq_dec X' X) then 
+      sp_mu X' phi'
+    else
+      sp_mu X' (e_subst_set phi' psi X)
 end.
 
-Definition var (name : string) : Sigma_pattern :=
-  sp_var (evar_c name).
+Definition var (name : string) : Sigma_pattern := sp_var (evar_c name).
 
-Definition set (name : string) : Sigma_pattern :=
-  sp_set (svar_c name).
-
-(* Check negb. *)
+Definition set (name : string) : Sigma_pattern := sp_set (svar_c name).
 
 Definition evar_eq (x y : EVar) : bool :=
-  match x, y with
-  | evar_c id_x, evar_c id_y => eqb id_x id_y
-  end
-.
+match x, y with
+| evar_c id_x, evar_c id_y => eqb id_x id_y
+end.
 
 Fixpoint free_vars (phi : Sigma_pattern) : (ListSet.set EVar) :=
-  match phi with
- | sp_var x => set_add evar_eq_dec x List.nil
- | sp_set X => List.nil
- | sp_const sigma => List.nil
- | sp_app phi1 phi2 =>
-    set_union evar_eq_dec
-      (free_vars phi1)
-      (free_vars phi2)
- | sp_bottom => List.nil
- | sp_impl phi1 phi2 =>
-    set_union evar_eq_dec
-      (free_vars phi1)
-      (free_vars phi2)
- | sp_exists y phi =>
+match phi with
+| sp_var x => set_add evar_eq_dec x List.nil
+| sp_set X => List.nil
+| sp_const sigma => List.nil
+| sp_app phi1 phi2 => set_union evar_eq_dec (free_vars phi1) (free_vars phi2)
+| sp_bottom => List.nil
+| sp_impl phi1 phi2 => set_union evar_eq_dec (free_vars phi1) (free_vars phi2)
+| sp_exists y phi => 
     set_diff evar_eq_dec
       (free_vars phi)
       (set_add evar_eq_dec y List.nil)
- | sp_mu X phi => free_vars phi
-end
-.
-
-(* Definition is_free (x : EVar) (phi : Sigma_pattern) : bool :=
-  set_mem evar_eq_dec x (free_vars phi). *)
-
-(* Inductive application_context : Set :=
-  | pattern (p : Sigma_pattern)
-  | box
-.
- *)
+| sp_mu X phi => free_vars phi
+end.
 
 Inductive context : Set :=
-  | box
-  | ctx_app_l (cc : context) (sp : Sigma_pattern)
-  | ctx_app_r (sp : Sigma_pattern) (cc : context)
+| box
+| ctx_app_l (cc : context) (sp : Sigma_pattern)
+| ctx_app_r (sp : Sigma_pattern) (cc : context)
 .
 
 Fixpoint subst_ctx (cc : context) (sp : Sigma_pattern) : Sigma_pattern :=
-  match cc with
-  | box => sp
-  | ctx_app_l cc' sp' => sp_app (subst_ctx cc' sp) sp'
-  | ctx_app_r sp' cc' => sp_app sp' (subst_ctx cc' sp)
-  end
-.
+match cc with
+| box => sp
+| ctx_app_l cc' sp' => sp_app (subst_ctx cc' sp) sp'
+| ctx_app_r sp' cc' => sp_app sp' (subst_ctx cc' sp)
+end.
 
-(* Definition box_context := subst_ctx box sp_bottom.
+(* Example of context usage: *)
+Definition box_context := subst_ctx box sp_bottom.
 Eval compute in box_context.
 
-Definition tree_context := subst_ctx (
-    ctx_app_l (ctx_app_r sp_bottom box) (sp_app sp_bottom sp_bottom)
-  ) sp_bottom.
-Eval compute in tree_context. *)
+Definition tree_context :=
+  subst_ctx
+    (ctx_app_l (ctx_app_r sp_bottom box) (sp_app sp_bottom sp_bottom))
+    sp_bottom.
+Eval compute in tree_context.
 
 Definition free_vars_ctx (C : context) : (ListSet.set EVar) :=
-  match C with
-  | box => List.nil
-  | ctx_app_l cc sp => free_vars sp
-  | ctx_app_r sp cc => free_vars sp
-  end
-.
-(* Inductive got_tau : Sigma_pattern -> Prop :=
-  | cons (phi : Sigma_partern) : got_tau (sp_impl sp_bottom phi)
-. *)
+match C with
+| box => List.nil
+| ctx_app_l cc sp => free_vars sp
+| ctx_app_r sp cc => free_vars sp
+end.
 
 Inductive got : Sigma_pattern -> Prop :=
-  (* Propositional tautology *)
-  | E_prop_tau1 (phi : Sigma_pattern) :
-      got (sp_impl phi phi)
+(* Propositional tautology *)
+| E_prop_tau1 (phi : Sigma_pattern) :
+    got (sp_impl phi phi)
 
-  | E_prop_tau2 (phi psi : Sigma_pattern) :
-      got (sp_impl phi (sp_impl psi phi))
+| E_prop_tau2 (phi psi : Sigma_pattern) :
+    got (sp_impl phi (sp_impl psi phi))
 
-  | E_prop_tau3 (phi psi xi : Sigma_pattern) :
-      got (
-        sp_impl
-          (sp_impl phi (sp_impl psi xi))
-          (sp_impl (sp_impl phi psi) (sp_impl phi xi)))
+| E_prop_tau3 (phi psi xi : Sigma_pattern) :
+    got
+      (sp_impl
+        (sp_impl phi (sp_impl psi xi))
+        (sp_impl (sp_impl phi psi) (sp_impl phi xi)))
 
-  | E_prop_tau4 (phi psi : Sigma_pattern) :
-      got (sp_impl
+| E_prop_tau4 (phi psi : Sigma_pattern) :
+    got
+      (sp_impl
         (sp_impl (sp_not phi) (sp_not psi))
         (sp_impl (psi) (psi)))
 
-  (* Modus ponens *)
-  | E_mod_pon (phi1 phi2 : Sigma_pattern) :
-    got phi1 ->
-    got (sp_impl phi1 phi2) ->
-    got phi2
+(* Modus ponens *)
+| E_mod_pon (phi1 phi2 : Sigma_pattern) :
+  got phi1 -> got (sp_impl phi1 phi2) -> got phi2
 
-  (* Existential quantifier *)
-  | E_ex_quan {phi : Sigma_pattern} (x y : EVar) :
-    got (sp_impl (e_subst_var phi (sp_var y) x) (sp_exists x phi))
+(* Existential quantifier *)
+| E_ex_quan {phi : Sigma_pattern} (x y : EVar) :
+  got (sp_impl (e_subst_var phi (sp_var y) x) (sp_exists x phi))
 
-  (* Existential generalization *)
-  | E_ex_gen (phi1 phi2 : Sigma_pattern) (x : EVar) :
-    got (sp_impl phi1 phi2) ->
-    negb (set_mem evar_eq_dec x (free_vars phi2)) = true ->
-    got (sp_impl (sp_exists x phi1) phi2)
+(* Existential generalization *)
+| E_ex_gen (phi1 phi2 : Sigma_pattern) (x : EVar) :
+  got (sp_impl phi1 phi2) ->
+  negb (set_mem evar_eq_dec x (free_vars phi2)) = true ->
+  got (sp_impl (sp_exists x phi1) phi2)
 
-  (* Propagation bottom *)
-  | E_prop_bot (C : context) :
-    got (sp_impl (subst_ctx C sp_bottom) sp_bottom)
+(* Propagation bottom *)
+| E_prop_bot (C : context) :
+  got (sp_impl (subst_ctx C sp_bottom) sp_bottom)
 
-  (* Propagation disjunction *)
-  | E_prop_dis (C : context) (phi1 phi2 : Sigma_pattern) :
-      (* phi3 = context cs (sp_or phi1 phi2) ->
-      phi4 = context cs phi1 ->
-      phi5 = context cs phi2 ->
-      got_c (sp_impl phi3 (sp_or phi4 phi5)) *)
-      got (sp_impl
-            (subst_ctx C (sp_or phi1 phi2))
-            (sp_or
-              (subst_ctx C phi1)
-              (subst_ctx C phi2)))
+(* Propagation disjunction *)
+| E_prop_dis (C : context) (phi1 phi2 : Sigma_pattern) :
+    (* phi3 = context cs (sp_or phi1 phi2) ->
+       phi4 = context cs phi1 ->
+       phi5 = context cs phi2 ->
+       got_c (sp_impl phi3 (sp_or phi4 phi5)) *)
+    got
+      (sp_impl
+        (subst_ctx C (sp_or phi1 phi2))
+        (sp_or
+          (subst_ctx C phi1)
+          (subst_ctx C phi2)))
 
-  (* Propagation exist *)
-  | E_prop_ex (C : context) (phi : Sigma_pattern) (x : EVar) :
-    negb (set_mem evar_eq_dec x (free_vars_ctx C)) = true ->
-    got (sp_impl
-      (subst_ctx C (sp_exists x phi))
-      (sp_exists x (subst_ctx C phi)))
+(* Propagation exist *)
+| E_prop_ex (C : context) (phi : Sigma_pattern) (x : EVar) :
+  negb (set_mem evar_eq_dec x (free_vars_ctx C)) = true ->
+  got (sp_impl
+    (subst_ctx C (sp_exists x phi))
+    (sp_exists x (subst_ctx C phi)))
 
-  (* Framing *)
-  | E_framing (C : context) (phi1 phi2 : Sigma_pattern) :
-    got (sp_impl phi1 phi2) ->
-    got (sp_impl (subst_ctx C phi1) (subst_ctx C phi2))
+(* Framing *)
+| E_framing (C : context) (phi1 phi2 : Sigma_pattern) :
+  got (sp_impl phi1 phi2) ->
+  got (sp_impl (subst_ctx C phi1) (subst_ctx C phi2))
 
-  (* Set Variable Substitution *)
-  | E_svar_subst (phi : Sigma_pattern) (psi X : SVar) :
-    got phi ->
-    got (e_subst_set phi (sp_set psi) X)
+(* Set Variable Substitution *)
+| E_svar_subst (phi : Sigma_pattern) (psi X : SVar) :
+  got phi -> got (e_subst_set phi (sp_set psi) X)
 
-  (* Pre-Fixpoint *)
-  | E_pre_fixp (phi : Sigma_pattern) (X : SVar) :
-    got (sp_impl
-          (e_subst_set phi (sp_mu X phi) X)
-          (sp_mu X phi))
+(* Pre-Fixpoint *)
+| E_pre_fixp (phi : Sigma_pattern) (X : SVar) :
+  got
+    (sp_impl
+      (e_subst_set phi (sp_mu X phi) X)
+      (sp_mu X phi))
 
-  (* Knaster-Tarski *)
-  | E_knaster_tarski (phi psi : Sigma_pattern) (X : SVar) :
-    got (sp_impl (e_subst_set phi psi X) psi) ->
-    got (sp_impl (sp_mu X phi) psi)
+(* Knaster-Tarski *)
+| E_knaster_tarski (phi psi : Sigma_pattern) (X : SVar) :
+  got (sp_impl (e_subst_set phi psi X) psi) -> got (sp_impl (sp_mu X phi) psi)
 
-  (* Existence *)
-  | E_existence (x : EVar) : got (sp_exists x (sp_var x))
+(* Existence *)
+| E_existence (x : EVar) : got (sp_exists x (sp_var x))
 
-  (* Singleton *)
-  | E_singleton (C1 C2 : context) (x : EVar) (phi : Sigma_pattern) :
-    got (sp_not (sp_and
-            (subst_ctx C1 (sp_and (sp_var x) phi))
-            (subst_ctx C2 (sp_and (sp_var x) (sp_not phi)))))
+(* Singleton *)
+| E_singleton (C1 C2 : context) (x : EVar) (phi : Sigma_pattern) :
+  got
+    (sp_not (sp_and
+      (subst_ctx C1 (sp_and (sp_var x) phi))
+      (subst_ctx C2 (sp_and (sp_var x) (sp_not phi)))))
 .
 
-(* Provability
-    - can be formalised with the M-valuation, "can be deduced" and can be proved operator
-*)
+(* Provability:
+ *  - can be formalised with the M-valuation
+ *  - "can be deduced" and "can be proved" operator *)
 
-(* Inductive proof_result : ? :=
+(* Inductive proof_result : Set :=
   | success (?)
   | fail
 . *)
 
 
-(* Definition 7., page 5. *)
-(* Definedness: *)
+(* Definition 7.: Definedness: *)
 Definition c_definedness := sp_const(sigma_c("definedness")).
-Definition Definedness (phi : Sigma_pattern) : Sigma_pattern := (c_definedness _._ phi).
+Definition Definedness (phi : Sigma_pattern) : Sigma_pattern :=
+  (c_definedness _._ phi).
 Notation "|^ phi ^|" := (Definedness phi) (at level 100).
 
 (* Totality *)
@@ -313,7 +296,6 @@ Notation "|_ phi _|" := (Totality phi).
 
 (* Equality *)
 Definition c_equality := sp_const(sigma_c("equality")).
-(* TODO: it is a legal interpretation? *)
 Definition Equality (l r : Sigma_pattern) := ((c_equality _._ l) _._ r).
 Notation "phi1 ~=~ phi2" := (Equality phi1 phi2) (at level 100).
 
@@ -322,24 +304,19 @@ Definition c_non_equality := sp_const(sigma_c("non-equality")).
 Definition NonEquality (l r : Sigma_pattern) := ((c_non_equality _._ l) _._ r).
 Notation "phi1 !=~ phi2" := (NonEquality phi1 phi2) (at level 100).
 
-(* Variable membership *)
+(* Membership *)
 Definition c_membership := sp_const(sigma_c("membership")).
-                      (* x can only be sp_var or sp_const *)
-                  (* this can be restricted with operational evaluation rules *)
-Definition Membership (x : Sigma_pattern) (phi : Sigma_pattern) := 
+(* - parameterx can only be sp_var or sp_const
+ * - this can be restricted with operational evaluation rules *)
+Definition Membership (x : Sigma_pattern) (phi : Sigma_pattern) :=
   ((c_membership _._ x) _._ phi).
 Notation "x -< phi" := (Membership x phi) (at level 100).
 
-(* Variable non-membership *)
+(* Non-membership *)
 Definition c_non_membership := sp_const(sigma_c("non-membership")).
 Definition NonMembership (x : EVar) (phi : Sigma_pattern) := 
   ((c_non_membership _._ (sp_var x)) _._ phi).
 Notation "x !-< phi" := (NonMembership x phi) (at level 100).
-
-(* Pattern non-membership *)
-(* Definition NonMembership (x : Sigma_pattern) (phi : Sigma_pattern) := 
-  ((c_non_membership _._ x) _._ phi).
-Notation "x !-< phi" := (NonMembership x phi) (at level 100). *)
 
 (* Set inclusion *)
 Definition c_set_incl := sp_const(sigma_c("set inclusion")).
@@ -375,14 +352,6 @@ Inductive OneStepTransition : Sigma_pattern -> Sigma_pattern -> Prop :=
     ((c_non_membership _._ x) _._ phi) |->
     (sp_not (Membership x phi))
 
-(* | OST_membership {x : Sigma_pattern} {phi : Sigma_pattern} :
-    ((c_membership _._ x) _._ phi) |->
-    (Totality (sp_and x phi))
-
-| OST_non_membership {x : Sigma_pattern} {phi : Sigma_pattern} :
-    ((c_non_membership _._ x) _._ phi) |->
-    (sp_not (Membership x phi)) *)
-
 | OST_set_inclusion {l r} :
     ((c_set_incl _._ l) _._ r) |->
     (Totality (sp_impl l r))
@@ -392,9 +361,9 @@ Inductive OneStepTransition : Sigma_pattern -> Sigma_pattern -> Prop :=
     (sp_not (SetInclusion l r))
 where "a |-> b" := (OneStepTransition a b).
 
-(* TODO: tests!!! *)
-(* Theorem test01 : (Totality (sp_bottom)) |-> (sp_not (Definedness (sp_not sp_bottom))).
-Proof. eapply OST_totality. Qed. *)
+Lemma test01 :
+  (Totality (sp_bottom)) |-> (sp_not (Definedness (sp_not sp_bottom))).
+Proof. eapply OST_totality. Qed.
 
 Reserved Notation "phi |->* phi'" (at level 100).
 Inductive AnyStepTransition : Sigma_pattern -> Sigma_pattern -> Prop :=
@@ -406,13 +375,13 @@ Inductive AnyStepTransition : Sigma_pattern -> Sigma_pattern -> Prop :=
     (phi |->* phi'')
 where "phi |->* phi'" := (AnyStepTransition phi phi').
 
-(* Theorem test02 : (Totality (sp_bottom)) |->* (sp_not (Definedness (sp_not sp_bottom))).
+Lemma test02 :
+  (Totality (sp_bottom)) |->* (sp_not (Definedness (sp_not sp_bottom))).
 Proof.
   eapply AST_trans.
   - eapply OST_totality.
   - eapply AST_refl.
-Qed. *)
-
+Qed.
 
 (* Many-sorted algebra *)
 Section MSA.
@@ -424,7 +393,7 @@ Inductive MSA_sorts : Set :=
 | Cfg
 .
 
-(* a function which corresponds constants of AML to sorts of MSA *)
+(* a function which corresponds: constants of AML  to  sorts of MSA *)
 Fixpoint AML_sort_name (s : MSA_sorts) : Sigma_pattern :=
 match s with
 | Nat => sp_const(sigma_c("Nat"))
@@ -439,7 +408,8 @@ Definition AML_Cfg := AML_sort_name(Cfg).
 
 
 Definition c_inhabitant_set := sp_const(sigma_c("inhabitant set")).
-Definition InhabitantSetOf (s : MSA_sorts) := (c_inhabitant_set _._ (AML_sort_name s)).
+Definition InhabitantSetOf (s : MSA_sorts) :=
+  (c_inhabitant_set _._ (AML_sort_name s)).
 Notation "'[[' s ']]'" := (InhabitantSetOf s) (at level 100).
 
 Definition vc := VectorDef.cons.
@@ -453,7 +423,8 @@ match n with
 | S n' => ((List.hd sp_bottom vec) _&_ (_and_gen n' (List.tl vec)))
 end.
 
-Fixpoint and_gen {n : nat} (vec : VectorDef.t Sigma_pattern n) : Sigma_pattern := 
+Fixpoint and_gen {n : nat} (vec : VectorDef.t Sigma_pattern n)
+: Sigma_pattern := 
   _and_gen n (to_list vec).
 
 Lemma zero_eq : (_and_gen 0 (List.nil)) = sp_bottom.
@@ -470,7 +441,8 @@ Lemma x1_eq' : (and_gen (vc _ x1 0 (vn _))) = x1.
 Proof. simpl. reflexivity. Qed.
 
 Definition x2 := sp_var(evar_c("x2")).
-Lemma x1_x2_eq : (_and_gen 2 ((List.cons x1) (List.cons x2 List.nil))) = (x1 _&_ x2).
+Lemma x1_x2_eq :
+  (_and_gen 2 ((List.cons x1) (List.cons x2 List.nil))) = (x1 _&_ x2).
 Proof. simpl. reflexivity. Qed.
 
 Lemma x1_x2_eq' : (and_gen (vc _ x1 1 (vc _ x2 0 (vn _)))) = (x1 _&_ x2).
@@ -478,72 +450,89 @@ Proof. simpl. reflexivity. Qed.
 
 Definition x3 := sp_var(evar_c("x3")).
 Lemma x1_x2_x3_eq :
-  (_and_gen 3 ((List.cons x1) ((List.cons x2) ((List.cons x3) List.nil))))
-= (x1 _&_ x2 _&_ x3).
+  (_and_gen 3 ((List.cons x1) ((List.cons x2) ((List.cons x3) List.nil)))) =
+  (x1 _&_ x2 _&_ x3).
 Proof. simpl. reflexivity. Qed.
 
 Definition x4 := sp_var(evar_c("x4")).
 Lemma x1_x2_x3__x4_eq :
-  (_and_gen 4 ((List.cons x1) (
-    (List.cons x2) ((List.cons x3) ((List.cons x4) List.nil)))))
-= (x1 _&_ x2 _&_ x3 _&_ x4).
+  (_and_gen 4 ((List.cons x1) 
+    ((List.cons x2) ((List.cons x3) ((List.cons x4) List.nil))))) =
+  (x1 _&_ x2 _&_ x3 _&_ x4).
 Proof. simpl. reflexivity. Qed.
 
-Fixpoint _assoc_elem (n : nat) (vars : list Sigma_pattern) (sorts : list MSA_sorts) : Sigma_pattern :=
+Fixpoint _assoc_elem (n : nat) (vars : list Sigma_pattern)
+                     (sorts : list MSA_sorts)
+: Sigma_pattern :=
 match n with
 | O => sp_bottom
-| S O => ((List.hd (sp_const (sigma_c("error at elem assoc S O"))) vars) -< [[ (List.hd Nat sorts) ]])
-| S n' => sp_and
-      ( (List.hd (sp_const (sigma_c("error at elem assoc S n"))) vars) -< [[ (List.hd Nat sorts) ]] )
+| S O => ((List.hd (sp_const (sigma_c("error at elem assoc S O"))) vars) -<
+          [[ (List.hd Nat sorts) ]])
+| S n' =>
+    sp_and
+      ((List.hd (sp_const (sigma_c("error at elem assoc S n"))) vars) -<
+       [[ (List.hd Nat sorts) ]])
       (_assoc_elem n' (List.tl vars) (List.tl sorts))
 end.
 
-Fixpoint assoc_elem {n : nat} (vars : VectorDef.t Sigma_pattern n) (sorts : VectorDef.t MSA_sorts n) : Sigma_pattern :=
+Fixpoint assoc_elem {n : nat} (vars : VectorDef.t Sigma_pattern n)
+                    (sorts : VectorDef.t MSA_sorts n)
+: Sigma_pattern :=
   _assoc_elem n (to_list (vars)) (to_list (sorts)).
 
 Lemma zero_eq_assoc : (_assoc_elem 0 (List.nil) (List.nil)) = sp_bottom.
 Proof. simpl. reflexivity. Qed.
 
 Lemma x1_eq_assoc : 
-  (_assoc_elem 1 ((List.cons x1) List.nil) ((List.cons Nat) List.nil))
-= (x1 -< [[ Nat ]]).
+  (_assoc_elem 1 ((List.cons x1) List.nil) ((List.cons Nat) List.nil)) = 
+  (x1 -< [[ Nat ]]).
 Proof. simpl. reflexivity. Qed.
 
 Lemma x1_x2_eq_assoc : 
   (_assoc_elem 2
     ((List.cons x1) (List.cons x2 List.nil))
-    ((List.cons Nat) (List.cons List List.nil)))
-= ((x1 -< [[ Nat ]]) _&_ (x2 -< [[ List ]])).
+    ((List.cons Nat) (List.cons List List.nil))) =
+  ((x1 -< [[ Nat ]]) _&_ (x2 -< [[ List ]])).
 Proof. simpl. reflexivity. Qed.
 
-Lemma x1_x2_x3_eq_assoc : 
-  (_assoc_elem 3 
+Lemma x1_x2_x3_eq_assoc :
+  (_assoc_elem 3
     ((List.cons x1) ((List.cons x2) (List.cons x3 List.nil)))
-    ((List.cons Nat) ((List.cons List) (List.cons Cfg List.nil))))
-= ((x1 -< [[ Nat ]]) _&_ (x2 -< [[ List ]]) _&_ (x3 -< [[ Cfg ]])).
+    ((List.cons Nat) ((List.cons List) (List.cons Cfg List.nil)))) =
+  ((x1 -< [[ Nat ]]) _&_ (x2 -< [[ List ]]) _&_ (x3 -< [[ Cfg ]])).
 Proof. simpl. reflexivity. Qed.
 
-Lemma x1_x2_x3__x4_eq_assoc : 
-  (_assoc_elem 4 
-    ((List.cons x1) ((List.cons x2) ((List.cons x3) (List.cons x4 List.nil))))
-    ((List.cons Nat) ((List.cons List) ((List.cons Cfg) (List.cons Nat List.nil)))))
-= ((x1 -< [[ Nat ]]) _&_ (x2 -< [[ List ]]) _&_ (x3 -< [[ Cfg ]]) _&_ 
-    (x4 -< [[ Nat ]])).
+Lemma x1_x2_x3__x4_eq_assoc :
+  (_assoc_elem 4
+    ((List.cons x1)
+      ((List.cons x2) ((List.cons x3) (List.cons x4 List.nil))))
+    ((List.cons Nat)
+      ((List.cons List) ((List.cons Cfg) (List.cons Nat List.nil))))) =
+  ((x1 -< [[ Nat ]]) _&_
+    (x2 -< [[ List ]]) _&_ (x3 -< [[ Cfg ]]) _&_ (x4 -< [[ Nat ]])).
 Proof. simpl. reflexivity. Qed.
 
-Fixpoint _assoc_params (f : Sigma_pattern) (n : nat) (vars : list Sigma_pattern) : Sigma_pattern :=
+Fixpoint _assoc_params (f : Sigma_pattern) (n : nat)
+                       (vars : list Sigma_pattern)
+: Sigma_pattern :=
 match n with
 | O => f
-| S O => (f _._ (List.nth O vars (sp_const (sigma_c("error singleton fun param list")))))
-| S n' => (_assoc_params f n' vars) _._ 
-            (List.nth n' vars (sp_const (sigma_c("error long fun param list"))))
+| S O =>
+    (f _._
+        (List.nth O vars
+            (sp_const (sigma_c("error singleton fun param list")))))
+| S n' => 
+    (_assoc_params f n' vars) _._
+        (List.nth n' vars (sp_const (sigma_c("error long fun param list"))))
 end.
 
-Fixpoint assoc_params (f : Sigma_pattern) {n : nat} (vars : VectorDef.t Sigma_pattern n) : Sigma_pattern :=
+Fixpoint assoc_params (f : Sigma_pattern) {n : nat}
+                      (vars : VectorDef.t Sigma_pattern n)
+: Sigma_pattern :=
   _assoc_params f n (to_list (vars)).
 
-Definition c'_f := sigma_c("fun").
-Definition fun_f   := sp_const(c'_f).
+Definition c_fun := sigma_c("fun").
+Definition fun_f   := sp_const(c_fun).
 Lemma zero_eq_par : (_assoc_params fun_f 0 (List.nil)) = fun_f.
 Proof. simpl. unfold fun_f. reflexivity. Qed.
 
@@ -552,13 +541,14 @@ Lemma x1_eq_par :
 Proof. simpl. unfold fun_f. unfold x1. reflexivity. Qed.
 
 Lemma x1_x2_eq_par :
-  (_assoc_params fun_f 2 ((List.cons x1) (List.cons x2 List.nil)))
-= (fun_f _._ x1 _._ x2).
+  (_assoc_params fun_f 2 ((List.cons x1) (List.cons x2 List.nil))) = 
+  (fun_f _._ x1 _._ x2).
 Proof. simpl. unfold fun_f. unfold x1. unfold x2. reflexivity. Qed.
 
 Lemma x1_x2_x3_eq_par :
-  (_assoc_params fun_f 3 ((List.cons x1) ((List.cons x2) (List.cons x3 List.nil))))
-= (fun_f _._ x1 _._ x2 _._ x3).
+  (_assoc_params fun_f 3
+    ((List.cons x1) ((List.cons x2) (List.cons x3 List.nil)))) = 
+  (fun_f _._ x1 _._ x2 _._ x3).
 Proof. simpl. unfold fun_f. unfold x1. unfold x2. unfold x3. reflexivity. Qed.
 
 Lemma x1_x2_x3__x4_eq_par :
@@ -570,17 +560,22 @@ Proof. simpl. reflexivity. Qed.
 
 Definition Nonempty_Sort (s : MSA_sorts) := ([[ s ]] !=~ sp_bottom).
 
-(* if constant function, then sp_bottom will stand on the application's left hand-side, because false implies everything *)
-(* this is allowed because this is only syntax and not the deduction - we don't need the type restriction at syntax level *)
-(* Definition __y := evar_c("__y"). (* we abstract away this variable. in fact it can be anything *) *)
+(* if constant function is defined, then sp_bottom will stand on the 
+ * application's left hand-side, because in the formalisation with Function
+ * axiom, a function traslates to an implication, and because of false implies
+ * everything, it imples the result too  *)
+(* this is allowed because this is only syntax and not the deduction - we don't 
+ * need the type restriction at syntax level *)
 Definition Function (f : Sigma_pattern) {n : nat}
             (ss : t MSA_sorts n) (s : MSA_sorts)
             (xs : t Sigma_pattern n) (y : EVar) : Sigma_pattern :=
   (sp_impl
-    (assoc_elem xs ss) (* ((x1 -< [[s1]]) _&_ .. _&_ (xn -< [[sn]])) *)
+    (* ((x1 -< [[s1]]) _&_ .. _&_ (xn -< [[sn]])) *)
+    (assoc_elem xs ss)
     (sp_exists y (sp_and
       ((sp_var y) -< [[ s ]])
-      ((assoc_params f xs) ~=~ (sp_var y)) (* ((f _._ x1) _._ .. _._ xn) ~=~ y *)))).
+      (* ((f _._ x1) _._ .. _._ xn) ~=~ y *)
+      ((assoc_params f xs) ~=~ (sp_var y)) ))).
 
 Definition Sort (s : MSA_sorts) := s.
 
@@ -600,14 +595,20 @@ Check (fun_f _:_ Nat X Nat --> Nat).
 
 (* Instead of notation "forall x : Nat . pattern" we introduce: *)
 Notation "'for_some' xc 'of_sort' sort 'states' pattern" := 
-  (sp_exists xc (sp_and ((sp_var xc) -< InhabitantSetOf(sort)) pattern)) (at level 0).
+  (sp_exists xc (sp_and ((sp_var xc) -< InhabitantSetOf(sort)) pattern))
+    (at level 0).
 Notation "'for_all' xc 'of_sort' sort 'states' pattern" := 
-  (sp_forall xc (sp_impl ((sp_var xc) -< InhabitantSetOf(sort)) pattern)) (at level 0).
+  (sp_forall xc (sp_impl ((sp_var xc) -< InhabitantSetOf(sort)) pattern))
+  (at level 0).
 
-(* Notation "'exists' xc : sort , pattern" := 
-(sp_exists xc (sp_and ((sp_var xc) -< InhabitantSetOf(sort)) pattern)) (at level 5, xc at next level, sort at next level, pattern at next level).
+(*
+Notation "'exists' xc : sort , pattern" := 
+  (sp_exists xc (sp_and ((sp_var xc) -< InhabitantSetOf(sort)) pattern)) (
+    at level 5, xc at next level, sort at next level, pattern at next level).
 Notation "'for_all' xc : sort , pattern" := 
-  (sp_forall xc (sp_impl ((sp_var xc) -< InhabitantSetOf(sort)) pattern)) (at level 0). *)
+  (sp_forall xc (sp_impl ((sp_var xc) -< InhabitantSetOf(sort)) pattern)) (
+    at level 5, xc at next level, sort at next level, pattern at next level).
+*)
 
 (* Proposition 18. *)
 Reserved Notation "a |--> b" (at level 40, left associativity).
@@ -620,7 +621,7 @@ Inductive QuantificationEquivalence : Sigma_pattern -> Sigma_pattern -> Prop :=
      (sp_not (for_some xc of_sort sort states (sp_not pattern))))
 where "a |--> b" := (QuantificationEquivalence a b).
 
-(* Natural numbers *)
+
 Section NaturalNumbers.
 
 Definition zero : Sigma_pattern := sp_const(sigma_c("zero")).
@@ -628,25 +629,16 @@ Definition succ : Sigma_pattern := sp_const (sigma_c("succ")).
 Definition plus : Sigma_pattern := sp_const (sigma_c("plus'")).
 Definition mult : Sigma_pattern := sp_const (sigma_c("mult")).
 
-(* Inductive Nat_elements : Type :=
-| zero (res_var : EVar) : ((c_zero _:_ --> Nat) (vn _) res_var)
-. *)
-
 Definition zero_fun := (zero _:_ --> Nat).
 Definition succ_fun := (succ _:_ Nat --> Nat).
 Definition plus_fun := (plus _:_ Nat X Nat --> Nat).
 Definition mult_fun := (mult _:_ Nat X Nat --> Nat).
 
-(* Definition zero''                       := zero_pat (vn _).
-Definition succ'' (x : Sigma_pattern)   := succ_pat (vc _ x 0 (vn _)).
-Definition plus'' (x y : Sigma_pattern) := plus'_pat (vc _ x 1 (vc _ y 0 (vn _))).
-Definition mult'' (x y : Sigma_pattern) := mult_pat (vc _ x 1 (vc _ y 0 (vn _))). *)
-
 Definition succ' (x : Sigma_pattern)   := succ _._ x.
 Definition plus' (x y : Sigma_pattern) := plus _._ x _._ y.
 Definition mult' (x y : Sigma_pattern) := mult _._ x _._ y.
 
-(* Example: x + 0 = x *)
+(* helper notations for the following examples *)
 Definition c_x := (evar_c("x")).
 Definition c_y := (evar_c("y")).
 Definition c_z := (evar_c("z")).
@@ -656,15 +648,14 @@ Definition x := (sp_var (evar_c("x"))).
 Definition y := (sp_var (evar_c("y"))).
 Definition z := (sp_var (evar_c("z"))).
 
-(* Check (for_some c_x of_sort Nat states sp_bottom). *)
-
+(* Example: x + 0 = x *)
 Definition x_plus'_0_eq_x :=
   (for_all c_x of_sort Nat states ((plus' x zero) ~=~ x)).
 
 (* Examples *)
 
 (* we have to specify the type of function parameters, because if not, the
-following statement about natural numbers also can be formalised: *)
+ * following statement about natural numbers also can be formalised: *)
 Definition foo := plus' plus zero.
 
 Definition one := succ' zero.
@@ -675,11 +666,13 @@ Definition six := succ' five.
 
 Definition plus_1_2_eq_3 := ((plus' one two) ~=~ three).
 Definition plus_1_plus_2_3_eq_6 := ((plus' one (plus' two three)) ~=~ six).
-Definition plus_1_plus_2_3_eq_1_plus_2_plus_3 := ((plus' one (plus' two three)) ~=~ (plus' one (plus' two three))).
+Definition plus_1_plus_2_3_eq_1_plus_2_plus_3 :=
+  ((plus' one (plus' two three)) ~=~ (plus' one (plus' two three))).
 Definition plus_1_plus_2_3_eq_1_plus_5 :=
   ((plus' one (plus' two three)) ~=~ (plus' one five)).
 Definition x_plus_2_plus_3_eq_x_plus_5 := 
-  (for_all c_x of_sort Nat states ((plus' (plus' x two) three) ~=~ (plus' x five))).
+  (for_all c_x of_sort Nat states (
+    (plus' (plus' x two) three) ~=~ (plus' x five))).
 Definition x_plus_3_eq_x_plus_3 :=
   (for_all c_x of_sort Nat states (plus' x three) ~=~ (plus' x three)).
 Definition x_plus_y_eq_x_plus_y :=
@@ -690,7 +683,7 @@ Definition plus_1_2 := plus' one two.
 Definition plus_2_3 := plus' two three.
 Definition plus_1_plus_2_3 :=  plus' one plus_2_3.
 Definition plus_1_plus_2_3_eq_plus_1_plus_2_3 :=
- plus_1_plus_2_3 ~=~ plus' one plus_2_3.
+  plus_1_plus_2_3 ~=~ plus' one plus_2_3.
 Definition plus_1_plus_2_3_eq_plus_1_plus_2_3' :=
   plus_1_plus_2_3 ~=~ plus_1_plus_2_3.
 Definition plus_1_plus_2_3_eq_plus_1_5 := plus_1_plus_2_3 ~=~ plus' one five.
@@ -728,8 +721,8 @@ Definition plus_x_plus_z_3_eq_y :=
 Fixpoint SumFromZeroTo (n : Sigma_pattern) : Sigma_pattern :=
 match n with
 | sp_const _ => zero
-(* succ _ *)
-| sp_app _ b => plus' (succ' b) (SumFromZeroTo b)
+      (* succ b *)
+| sp_app _    b => plus' (succ' b) (SumFromZeroTo b)
 | _ => sp_const(sigma_c("non-exhaustive pattern"))
 end.
 
@@ -744,15 +737,16 @@ Proof. simpl. reflexivity. Qed.
 
 
 (* 1 + ... + n = n * (n+1) / 2. *)
-Definition Sum_of_first_n := 
-  for_all c_n of_sort Nat states (mult' two (SumFromZeroTo n) ~=~ mult' n (succ' n)).
+Definition Sum_of_first_n : Sigma_pattern :=
+  for_all c_n of_sort Nat states (mult' two (SumFromZeroTo n) ~=~
+  mult' n (succ' n)).
 
 
 Fixpoint ProdFromOneTo (n : Sigma_pattern) : Sigma_pattern :=
 match n with
 | sp_const _ => zero
-(* succ _ *)
-| sp_app a b => 
+      (* succ _ *)
+| sp_app _    b => 
   match b with
   | sp_const _ => one
   | sp_app _ _ => mult' (succ' b) (ProdFromOneTo b)
@@ -777,8 +771,8 @@ Proof. simpl. reflexivity. Qed.
 Fixpoint SumOfSquaresFromZeroTo (n : Sigma_pattern) : Sigma_pattern :=
 match n with
 | sp_const _ => zero
-(* succ _ *)
-| sp_app _ b => plus' (mult' (succ' b) (succ' b)) (SumOfSquaresFromZeroTo b)
+      (* succ b *)
+| sp_app _    b => plus' (mult' (succ' b) (succ' b)) (SumOfSquaresFromZeroTo b)
 | _ => sp_const(sigma_c("non-exhaustive pattern"))
 end.
 
@@ -788,7 +782,9 @@ Proof. simpl. reflexivity. Qed.
 Lemma until_one'' : (SumOfSquaresFromZeroTo one) = (plus' (mult' one one) zero).
 Proof. simpl. reflexivity. Qed.
 
-Lemma until_two'' : (SumOfSquaresFromZeroTo two) = (plus' (mult' two two) (plus' (mult' one one) zero)).
+Lemma until_two'' :
+  (SumOfSquaresFromZeroTo two) =
+  (plus' (mult' two two) (plus' (mult' one one) zero)).
 Proof. simpl. reflexivity. Qed.
 
 
@@ -803,17 +799,23 @@ End NaturalNumbers.
 
 Section MatchingMuLogic.
 
-Fixpoint _app_inhabitant_sets (n : nat) (vec : list MSA_sorts) : Sigma_pattern :=
+Fixpoint _app_inhabitant_sets (n : nat) (vec : list MSA_sorts)
+: Sigma_pattern :=
 match n with
 | O => sp_const (sigma_c("cannot operate on empty parameters"))
 | S O => InhabitantSetOf (List.hd Nat vec)
-| S n' => InhabitantSetOf (List.hd Nat vec) _._ (_app_inhabitant_sets n' (List.tail vec))
+| S n' =>
+    InhabitantSetOf (List.hd Nat vec) _._
+    (_app_inhabitant_sets n' (List.tail vec))
 end.
 
-Fixpoint app_inhabitant_sets {n : nat} (vec : VectorDef.t MSA_sorts n) : Sigma_pattern :=
+Fixpoint app_inhabitant_sets {n : nat} (vec : VectorDef.t MSA_sorts n)
+ : Sigma_pattern :=
   _app_inhabitant_sets n (to_list vec).
 
-Lemma nil_eq_nil : app_inhabitant_sets (vn MSA_sorts) = sp_const (sigma_c("cannot operate on empty parameters")).
+Lemma nil_eq_nil : 
+  app_inhabitant_sets (vn MSA_sorts) =
+  sp_const (sigma_c("cannot operate on empty parameters")).
 Proof. simpl. reflexivity. Qed.
 
 Lemma app_inhabitant_sets_test_one_element :
@@ -821,16 +823,23 @@ Lemma app_inhabitant_sets_test_one_element :
 Proof. simpl. reflexivity. Qed.
 
 Lemma app_inhabitant_sets_test_two_elements :
-  (app_inhabitant_sets (vc _ Nat 1 (vc _ List 0 (vn _))) = (InhabitantSetOf(Nat) _._ InhabitantSetOf(List))).
+  (app_inhabitant_sets (vc _ Nat 1 (vc _ List 0 (vn _))) =
+  (InhabitantSetOf(Nat) _._ InhabitantSetOf(List))).
 Proof. simpl. reflexivity. Qed.
 
 Lemma app_inhabitant_sets_test_three_elements :
-  (app_inhabitant_sets (vc _ Nat 2 (vc _ List 1 (vc _ Cfg 0 (vn _)))) = (InhabitantSetOf(Nat)  _._ (InhabitantSetOf(List) _._ InhabitantSetOf(Cfg)))).
+  (app_inhabitant_sets (vc _ Nat 2 (vc _ List 1 (vc _ Cfg 0 (vn _)))) =
+  (InhabitantSetOf(Nat)  _._ (InhabitantSetOf(List) _._ InhabitantSetOf(Cfg)))).
 Proof. simpl. reflexivity. Qed.
 
                   (* sp_const only *)
-Definition Arity (sigma : Sigma_pattern) {n : nat} (s_vec : VectorDef.t MSA_sorts n) (s : MSA_sorts) :=
+Definition Arity (sigma : Sigma_pattern) {n : nat}
+                 (s_vec : VectorDef.t MSA_sorts n) (s : MSA_sorts)
+: Sigma_pattern :=
   sigma _._ (app_inhabitant_sets s_vec) <: InhabitantSetOf(s).
+
+(* Other equivalences of expressions, respectively equivalence validation are
+ * described in Theorem 21. *)
 
 End MatchingMuLogic.
 
@@ -851,8 +860,9 @@ End ConstructorsAndTermAlgebras.
 
 Section NaturalNumbers.
 
-
-Definition Inductive_Domain (D : SVar) := 
+(* here is applied perhaps pointwise application, which is interpreted in the
+ * denotational semantics *)
+Definition Inductive_Domain (D : SVar) :=
   (InhabitantSetOf(Nat)) ~=~ sp_mu D (sp_or zero (succ' (sp_set D))).
 
 Definition Peano_Induction (cn : EVar) (phi : Sigma_pattern -> Sigma_pattern) :=
@@ -884,7 +894,6 @@ Definition every_number_is_positive : Sigma_pattern :=
   Peano_Induction c_n (less_or_equal zero).
 
 Definition less2 (a b : Sigma_pattern) := less a (succ' b).
-(* indukcioval leirhato, hogy ha 0+1 > 0 és minden n>0-ra n+1 > 0 akkor n+1 > 0 *)
 
 (* States that if:
   - zero < zero + 1 and
